The following axioms were extract from [cite:@hodel2013introduction]:

- /Language:/ The symbols of the language are:

  - \(p_1, p_2, p_3, \dots\): An infinite list of propositional
    variables

  - \(\neg, \imp, \land, \lor\): negation, implication, conjunction, and
    disjunction symbol

  - \((, )\): left and right parenthesis for punctuation

- /Axioms:/

  - J1: \(A \imp (B \imp A)\)

  - J2: \((A \imp (B \imp C)) \imp ((A \imp B) \imp (A \imp C))\)

  - J3: \(A \land B \imp A\)

  - J4: \(A \land B \imp B\)

  - J5: \(A \imp (B \imp (A \land B))\)

  - J6: \(A \imp (A \lor B)\)

  - J7: \(B \imp (A \lor B)\)

  - J8: \((A \imp C) \imp ( ( B \imp C) \imp (( A \lor B) \imp C))\)

  - J9: \((A \imp B) \imp (( A \imp \neg B) \imp \neg A)\)

  - J10: \(\neg A \imp (A \imp B)\)

- /Rules of Inference:/

  - Modus Ponens:

    []B

As in classical logic \(A \dimp B\) is abbreviated as
\((A \imp B) \land (B \imp A)\). It is important to mention that the
other connective symbols do not share similar abbreviations as in the
classical counterpart. Since \(J\) as a formal system contains \(J1\)
and Modus Ponens as unique rule of inference, by the comment on Theorem
3 in Section 3.5 of [cite:@hodel2013introduction] we have that \(J\)
satisfies the Deduction theorem. A proof of the above is shown in the
next theorem:

(Deduction theoreom for \(J\)) If \(\Gamma \cup \{ A \} \vdash_J B\),
then \(\Gamma \vdash_J A \imp B\)

/Proof./ We proceed by induction on the number of steps in the proof of
\(B\) using \(\Gamma \cup \{A\}\). Assume
\(\Gamma \cup \{A \} \vdash_J B\), to prove
\(\Gamma \vdash_J A \imp B\). There are three cases:

- \(B\) is an axiom of \(J\) or \(B \in \Gamma\): From this we have that
  \(\vdash_J B\) Since \(J\) has \(J1\), we can conclude that
  \(\Gamma \vdash_J B \imp (A \imp B)\). By Modus Ponens we obtain
  \(\Gamma \vdash_J A \imp B\)

- \(B\) is in \(A\): In this case, the following is proof of
  \(\Gamma \vdash_J A \imp A\).

  - 1. \(A \imp (A \imp A)\), Axiom \(J1\)

  - 2. \(A \imp ((A \imp A) \imp A)\), Axiom \(J1\)

  - 3.
    \((A \imp ((A \imp A) \imp A)) \imp ( (A \imp (A \imp A)) \imp (A \imp A))\),
    Axiom \(J2\)

  - 4. \((A \imp (A \imp A)) \imp (A \imp A)\), Modus Ponens(2, 3)

  - 5. \(A \imp A\), Modus Ponens(1, 4)

- \(B\) is obtained from \(C\) and \(C \imp B\) by an application of
  Modus Ponens. By induction, we have from
  \(\Gamma \cup \{ A \} \vdash_J B\) and
  \(\Gamma \cup \{ A \} \vdash_J C \imp B\) the following
  \(\Gamma \vdash_J A \imp B\) and
  \(\Gamma \vdash_J A \imp (C \imp B)\). By \(J2\) we have that
  \(\Gamma \vdash_J (A \imp (C \imp B)) \imp ((A \imp B) \imp (A \imp C))\).
  A double application of Modus Ponens, we obtain
  \(\Gamma \vdash_J A \imp C\).

 ◻

\(\neg A \lor A\) and \(\neg \neg A \imp A\) are not theorems of \(J\).

/Proof./ Let us introduce an \(n+1\)-valued logic as follows: A truth
assignment is a function \(\phi : PROP \imp \{0, 1, \dots, n\}\); such
an assignment extends to all formulas \(FOR(\neg, \lor, \land, \imp)\)
of \(J\) according to these rules:

- \(\phi(A \lor B) = \min \{ \phi(A), \phi(B) \}\)

- \(\phi(\neg A) =  \begin{cases} 
          0 & \phi(A) = n \\
          n & \phi(A) < n
        \end{cases}\)

- \(\phi(A \land B) = \max \{ \phi(A), \phi(B) \}\)

- \(\phi(A \imp B) =  \begin{cases} 
          0 & \phi(A) \geq \phi(B) \\
          \phi(B) & \phi(A) < \phi(B)
        \end{cases}\)

We will prove that for every theorem \(A\) in \(J\) we have that
\(\phi(A) = 0\) by induction on the length of the proof:

- Base case: Since the base case accounts to axioms in \(J\), we need to
  prove that every axiom in \(J\) evaluates to 0 under \(\phi\):

  - Case \(J1\): Since \(\phi(A) \geq \phi(A)\) and \(\phi(A) \geq 0\)
    we have that \(\phi(A) \geq \phi(B \imp A)\), so
    \(\phi(A \imp (B \imp A)) = 0\).

  - Case \(J2\): To prove
    \(\phi(( A \imp (B \imp C)) \imp ((A \imp B) \imp (A \imp C))) = 0\).

    - Case 1. \(\phi(A) \geq \phi(B \imp C)\). This implies
      \(\phi(A \imp (B \imp C)) = 0\). Thus, it is enough to prove that
      \(\phi((A \imp B) \imp (A \imp C)) = 0\), i.e.
      \(\phi(A \imp B) \geq \phi(A \imp C)\).

      - Subcase 1. \(\phi(A) \geq \phi(B)\) and
        \(\phi(A) \geq \phi(C)\): This holds since \(0 \geq 0\).

      - Subcase 2. \(\phi(A) \geq \phi(B)\) and \(\phi(A) < \phi(C)\):
        It is enough to prove \(0 \geq \phi(C)\), i.e. \(\phi(C) = 0\).
        Suppose by contradiction that \(\phi(C) \neq 0\). We have that
        \(\phi(C) > \phi(A) \geq \phi(B)\), so \(\phi(C) > \phi(B)\).
        This implies that \(\phi(B \imp C) = \phi(C)\). Since
        \(\phi(A) \geq \phi(B \imp C)\) we have that
        \(\phi(A) \geq \phi(C)\). Therefore,
        \(\phi(C) > \phi(A) \geq \phi(C)\), a contradiction.

      - Subcase 3. \(\phi(A) < \phi(B)\) and \(\phi(A) \geq \phi(C)\):
        This holds since \(\phi(B) \geq 0\).

      - Subcase 4. \(\phi(A) < \phi(B)\) and \(\phi(A) < \phi(C)\): To
        prove that \(\phi(B) \geq \phi(C)\). Suppose by contradiction
        that \(\phi(B) < \phi(C)\), thus \(\phi(B \imp C) = \phi(C)\).
        Since \(\phi(A) \geq
                          \phi(B \imp C)\) we have that
        \(\phi(A) \geq \phi(C)\). Since
        \(\phi(C) > \phi(A) \geq \phi(C)\) we reach a contradiction.

    - Case 2. \(\phi(A) < \phi(B \imp C)\). The latter implies that
      \(\phi(A \imp (B \imp C)) = \phi(B \imp C)\). Hence, it is enough
      to prove that
      \(\phi(B \imp C) \geq \phi((A \imp B) \imp (A \imp C))\).

      - Subcase 1. \(\phi(B) \geq \phi(C)\): From the latter we have
        that \(\phi(B \imp C) = 0\). Hence, \(\phi(A) < 0\), but
        \(\phi(A) \geq 0\), a contradiction.

      - Subcase 2. \(\phi(B) < \phi(C)\): It is enough to prove that
        \(\phi(C) \geq \phi((A \imp B) \imp (A \imp C))\). Since
        \(\phi(B) < \phi(C)\) we have that \(\phi(B \imp C) = \phi(C)\).
        Since \(\phi(A) < \phi(B \imp C)\) we can conclude that hence
        \(\phi(C) > \phi(A)\).

        Let us prove the following observation : For any two formulas
        \(A, B \in 
                          FOR(\neg, \land, \lor, \imp)\), we have that
        \(\phi(A) \geq \phi(B \imp A)\). This happens because
        \(\phi(A) \geq 0\) and \(\phi(A) \geq 0\) and by definition of
        we have that \(\phi(B \imp A)\) is either \(0\) or \(\phi(A)\).

        From this observation we have that
        \(\phi(A \imp C) \leq \phi((A \imp B) \imp (A \imp C))\). Since
        \(\phi(A \imp C) = \phi(C)\) we can conclude that
        \(\phi(C) \geq \phi((A \imp B) \imp (A \imp C))\).

  - Case \(J3\): This follows from
    \(\max \{ \phi(A), \phi(B) \} \geq \phi(A)\).

  - Case \(J4\): This follows from
    \(\max \{ \phi(A), \phi(B) \} \geq \phi(B)\).

  - Case \(J5\): We notice the following cases:

    - Case \(\phi(A) < \phi(B) = \max \{ \phi(A), \phi(B) \}\): This
      reduces \(\phi(A \imp (B \imp A \land B)) = 0\) to check that
      \(\phi(A) \geq 0\), which is true.

    - Case \(\phi(B) < \phi(A) = \max \{ \phi(A), \phi(B) \}\): This
      reduces \(\phi(A \imp (B \imp A \land B)) = 0\) to check that
      \(\phi(A) \geq \max\{ \phi(A), \phi(B) \}\), which is true since
      \(\phi(A) = \max \{ \phi(A), \phi(B) \}\).

    - Case \(\phi(A) = \phi(B) = \max \{ \phi(A), \phi(B) \}\): This
      reduces \(\phi(A \imp (B \imp A \land B)) = 0\) to check that
      \(\phi(A) \geq 0\) which is true.

  - Case \(J6\): This follows from
    \(\min \{ \phi(A), \phi(B) \} \leq \phi(A)\).

  - Case \(J7\): This follows from
    \(\min \{ \phi(A), \phi(B) \} \leq \phi(A)\).

  - Case \(J8\): To prove that
    \(\phi((A \imp C) \imp ((B \imp C) \imp ((A \lor B) \imp C))) = 0\).

    - Case 1. \(\phi(A) \geq \phi(C)\): It is enough to prove that
      \(\phi((B \imp C) \imp ( ( A \lor B) \imp C)) = 0\), i.e.
      \(\phi(B \imp C) \geq \phi((A \lor B) \imp C)\).

      - Subcase 1. \(\phi(B) \geq \phi(C)\). It is enough to prove that
        \(\phi(A \lor B) \geq \phi(C)\). Since \(\phi(A) \geq \phi(C)\)
        and \(\phi(B) \geq \phi(C)\) then
        \(\phi(A \lor B) = \min \{ \phi(A), \phi(B) \} \geq \phi(C)\).

      - Subcase 2. \(\phi(B) < \phi(C)\). Since
        \(\phi(A) \geq \phi(C) > \phi(B)\) we conclude that
        \(\phi(A \lor B) = \phi(B)\). Because \(\phi(B) < \phi(C)\), we
        have that \(\phi(B \imp C) = \phi(C)\). Using the previous
        observation [[#observation][[observation]]] we have that
        \(\phi(C) \geq \phi((A \lor B) \imp C)\), thus
        \(\phi(B \imp C) \geq \phi((A \lor B) \imp C)\).

    - Case 2. \(\phi(A) < \phi(B \imp C)\).

      We will prove the following observation :
      \(\phi((A \land B) \imp C) = \phi(A \imp (B \imp C))\).

      - Case 1. \(\phi(A) \geq \phi(B \imp C)\): This means that
        \(\phi(A \imp (B \imp C)) = 0\), hence we need to prove that
        \(\phi((A \land B) \imp C) = 0\). We can see that
        \(\phi(A \imp (B \imp C)) = 0\) implies that
        \(\phi(A) \geq \phi(B \imp C)\), which means that if
        \(\phi(B) < \phi(C)\) we have that
        \(\phi(A) \geq \phi(B \imp C) = \phi(C)\). Suppose by
        contradiction that \(\phi((A \land B) \imp C) \neq 0\), so
        \(\phi(A \land B) < \phi(C) \neq 0\). Thus,
        \(\phi(C) > \phi(A)\) and \(\phi(C) > \phi(B)\). The latter
        entails \(\phi(A) \geq \phi(C) > \phi(A)\), a contradiction.

      - Case 2. \(\phi(A) < \phi(B \imp C)\): This implies that
        \(\phi(A \imp (B \imp C)) = \phi(B \imp C)\). So we need to
        prove that \(\phi((A \land B) \imp C) = \phi(B \imp C)\). We
        notice that \(\phi(B) < \phi(C)\), otherwise
        \(\phi(B \imp C) = 0\) so \(\phi(A) < 0\), a contradiction. From
        this, we conclude that \(\phi(B \imp C) = \phi(C)\), which
        reduces proving \(\phi(A \imp (B \imp C)) = \phi(B \imp C)\) to
        prove \(\phi(A \imp (B \imp C)) = \phi(C)\) instead. Since
        \(\phi(A) < \phi(B \imp C) = \phi(C)\), we have that
        \(\phi(C) > \max \{\phi(A), \phi(B) \}\). Therefore,
        \(\phi((A \land B) \imp C) = \phi(C)\) as desired.

      Returning to our original problem, we have that
      \(\phi(A) < \phi(B \imp C)\), hence it is enough to prove
      \(\phi(A) \geq \phi((B \imp C) \imp ((A \lor B) \imp C))\). From
      our previous observation [[#observation2][[observation2]]], we
      notive that
      \(\phi(A) \geq \phi(((B \imp C) \land (A \lor B)) \imp C)\), so by
      our first observation [[#observation][[observation]]] the latter
      is true.

  - Case \(J9\): To prove
    \(\phi((A \imp B) \imp ((A \imp \neg B) \imp \neg A)) = 0\), i.e
    \(\phi(A \imp B) \geq \phi((A \imp \neg B) \imp \neg A)\).

    - Case 1. \(\phi(A) \geq \phi(B)\): To prove
      \(\phi((A \imp \neg B) \imp \neg A) = 0\), i.e.
      \(\phi(A \imp \neg B) \geq \phi(\neg A)\).

      - Subcase 1. \(\phi(A) \geq \phi(\neg B)\): Since
        \(\phi(A) \geq \phi(B)\) and \(\phi(A) \geq \phi(\neg B)\) we
        conclude that \(\phi(A) = n\), thus \(\phi(\neg A) = 0\), so
        \(\phi(A \imp \neg B) \geq \phi(\neg A)\) reduces to
        \(0 \geq 0\) which is true.

      - Subcase 2. \(\phi(A) < \phi(\neg B)\): This reduces
        \(\phi(A \imp \neg B) \geq \phi(\neg A)\) to prove
        \(\phi(\neg B) \geq \phi(\neg A)\). Since
        \(\phi(A) \geq \phi(B)\) we have that
        \(\phi(\neg B) > \phi(B)\). This implies that
        \(\phi(\neg B) = n\), otherwise \(\phi(\neg B) = 0\) and
        \(\phi(B) = n\), but it cannot be the case that
        \(\phi(\neg B) > n\). The latter reduces
        \(\phi(\neg B) \geq \phi(\neg A)\) to prove
        \(n \geq \phi(\neg A)\) which is true.

    - Case 2. \(\phi(A) < \phi(B)\): This means that
      \(\phi(A \imp B) = \phi(B)\). To prove that
      \(\phi(B) \geq \phi((A \imp \neg B) \imp \neg A)\).

      - Subcase 1. \(\phi(A \imp \neg B) \geq \phi(\neg A)\). This means
        that \(\phi((A \imp \neg B) \imp \neg A) = 0\), which reduces
        \(\phi(B) \geq \phi((A \imp \neg B) \imp \neg A)\) to
        \(\phi(B) \geq 0\) which is true.

      - Subcase 2. \(\phi(A \imp \neg B) < \phi(\neg A)\). The latter
        means that \(\phi((A \imp \neg B) \imp \neg A) = \phi(\neg A)\).
        To prove \(\phi(B) \geq \phi(\neg A)\).

        Suppose by contradiction that \(\phi(B) < \phi(\neg A)\). Since
        \(\phi(A) \geq \phi(B)\) we have that
        \(\phi(\neg A) > \phi(A)\). So \(\phi(\neg A) = n\), otherwise
        \(\phi(A) = n\) and \(\phi(\neg A) > n\), which is not possible.
        The latter also entails that \(\phi(A) < n\). Additionally,
        \(\phi(B) < n\), otherwise \(n < \phi(\neg A)\), which is not
        possible. From the latter \(\phi(\neg B) = n\). Since
        \(\phi(A) < n = \phi(\neg B)\), we have that
        \(\phi(A \imp \neg B) = \phi(\neg B) = n\). But this implies
        that \(n > n\), a contradiction.

  - Case \(J10\): To prove that \(\phi(\neg A \imp (A \imp B)) = 0\),
    i.e. \(\phi(\neg A) \geq \phi(A \imp B)\).

    - Subcase 1. \(\phi(A) \geq \phi(B)\): So \(\phi(A \imp B) = 0\), so
      \(\phi(\neg A) \geq \phi(A \imp B)\) reduces to
      \(\phi(\neg A) \geq 0\), which is true.

    - Subcase 2. \(\phi(A) < \phi(B)\): This implies that
      \(\phi(A) < n\), otherwise \(n < \phi(B)\), which is not possible.
      Additionally, \(\phi(A \imp B) = \phi(B)\). Since \(\phi(A) < n\)
      we have that \(\phi(\neg A) = n\), thus
      \(\phi(\neg A) \geq \phi(A \imp B)\) reduces to
      \(n > \phi(A \imp B)\) which is true.

- Inductive case: Let \(\langle A_1, A_2, \dots, A_n, A_{n+1} \rangle\)
  be proof in \(J\) of size \(n+1\). We notice that the subproof
  \(\langle A_1, A_2, \dots, A_n \rangle\) satisfies the Inductive
  hypothesis, i.e. \(\phi(A_i) =\) for every \(1 \leq i \leq n\). We
  need to show that \(\phi(A_{n+1}) = 0\). Several cases are noticed:

  - \(A_{n+1}\) is an axiom of \(J\). Then by the base case we have that
    \(\phi(A_{n+1}) = 0\) as desired.

  - \(A_{n+1}\) was obtained using Modus Ponens using some
    \(A_i, A_j := A_i \imp A_{n+1}\) in the proof with \(i, j \leq n\).
    By the inductive hypothesis, we have that \(\phi(A_i) = 0\) and
    \(\phi(A_i \imp A_{n+1}) = 0\), which means that
    \(0 = \phi(A_i) \geq \phi(A_{n+1})\), thus \(\phi(A_{n+1}) = 0\).

With this invariant we conclude that \(\phi(A) = 0\) for every
\(\vdash_J A\). ◻

We notice that with an assignment \(\phi : PROP \imp \{0, 1, 2\}\) such
that \(\phi(A) = 1\) we have that
\(\phi(\neg A \lor A) = \min \{ \phi(\neg A), \phi(A) \}
= \min \{ 2 ,  1 \} = 1\). Additionally, \(\phi(\neg \neg A) = 0\) since
\(\phi(\neg A) = 2\), so \(\phi(\neg \neg A \imp A) = 1\) since
\(0 = \phi(\neg \neg A) < \phi(A) = 1\).

It is important to notice that the \(n+1\)-valued logic introduced in
the previous theorem can be considered and /invariant/ for the
propositional intuitionisc formal system. However, this truth assignment
does not constitute a semantics for the system \(J\). In fact, there are
no finite smeantics for intuitionistic logic as we will observe with the
following theorem:

For \(n \geq 2\), let \(D_n\) denote the formula:

#+begin_center
| \((p_1 \dimp p_2)\) | \(\lor\) | \((p_1 \dimp p_3)\) | \(\lor\) | \(\dots\) | \(\lor\) | \((p_1 \dimp p_n)\)     |
|                     | \(\lor\) | \((p_2 \dimp p_3)\) | \(\lor\) | \(\dots\) | \(\lor\) | \((p_2 \dimp p_n)\)     |
|                     |          |                     |          |           | \(\lor\) | \((p_{n-1} \dimp p_n)\) |

#+end_center

We have that \(\not \vdash_J D_n\).

/Proof./ We use the \(n+1\)-valued logic previously defined in theorem
[[#theorem1][[theorem1]]]. We notice that
\(\phi(D_n) = \min_{1 \leq i<j \leq n} \{ \phi(p_i \dimp p_j) \}\). Let
us suppose by contradiction that \(\vdash_J D_n\). Thus, by theorem
[[#theorem1][[theorem1]]] we have that \(\phi(D_n) = 0\), so there are
\(1 \leq i<j \leq n\) such that \(\phi(p_i \dimp p_j) = 0\). Since
\(p_i \dimp p_j\) stands for \((p_i \imp p_j) \land (p_i \imp p_j)\) we
have that \(\max \{ \phi(p_i \imp p_j), \phi(p_j \imp p_i) \} = 0\). The
latter implies that \(\phi(p_i \imp p_j) = 0\) and
\(\phi(p_j \imp p_i) = 0\), which entail that
\(\phi(p_i) \geq \phi(p_j)\) and \(\phi(p_j) \geq \phi(p_i)\). These
inequalities can be combined into \(\phi(p_i) = \phi(p_j)\). So if we
pick a truth assignment such that \(\phi(p_i) = i\) we notice that
\(D_n\) does not hold for all truth assignments in the \(n+1\)-valued
logic. ◻

Consider the language with connectives \(\neg, \lor, \land, \imp\). A
/matrix/ for this language is a 6-tuple \(M = 
  \langle S, S_0, H_\neg, H_\lor, H_\land, H_\imp \rangle\), where \(S\)
is a nonempty set whose elements are called /truth values/, \(S_0\) is a
subset of \(S\) whose elements are called /designated values/, and
\(H_\lor, H_\land, H_\imp\), and \(H_\neg\) are truth functions for
\(\lor, \land, \imp\), and \(\neg\). A /truth assignment/ for \(M\) is a
function \(\phi : PROP \imp S\). Such an assignment extends
\(FOR(\neg, \lor, \land, \imp)\) in the usual way.

There is no matrix \(M\) with \(S\) finite such that for every formula
\(A\), \(\vdash_J A \Leftrightarrow \phi(A) \in S_0\) for every truth
assignment \(\phi\) for \(M\).

/Proof./ Let us assume by contradiction that such matrix \(M\) exists
with \(n\) elements. We realize that \(D_{n+1}\) is not a theorem of
\(J\) from lemma [[#wow][[wow]]], so there is a truth assignment
\(\phi\) for \(M\) such that \(\phi(D_{n+1}) \not \in S_0\). By the
pigeonhole principle, there are \(1 \leq j < k \leq n+1\) such that
\(\phi(p_i) = \phi(p_k)\), i.e. more propositional variables than truth
values. Let \(E_{n+1} = D_{n+1}\) be obtained from \(D_{n+1}\) by
replacing \((p_j \dimp p_k)\) with \((p_k \dimp p_k)\). Since
\(\phi(p_j \dimp p_k) = H_\dimp(\phi(p_j), \phi(p_k))\) and \(H_\dimp\)
is a truth function, we have that
\(H_\dimp(\phi(p_j), \phi(p_k)) = H_\dimp(\phi(p_k), \phi(p_k))\) since
\(\phi(p_k) = \phi(p_j)\). So
\(H_\dimp(\phi(p_k), \phi(p_k)) = \phi(p_k \dimp p_k)\). Thus
\(\phi(D_{n+1}) = \phi(E_{n+1})\).

Let us prove the following theorem in \(J\): \(\vdash_J p_k \dimp p_k\).

- 1. \(p_k \imp (p_k \imp p_k)\), Axiom \(J1\)

- 2. \(p_k \imp ((p_k \imp p_k) \imp p_k)\), Axiom \(J1\)

- 3.
  \((p_k \imp ((p_k \imp p_k) \imp p_k)) \imp ( (p_k \imp (p_k \imp p_k)) \imp (p_k \imp p_k))\),
  Axiom \(J2\)

- 4. \((p_k \imp (p_k \imp p_k)) \imp (p_k \imp p_k)\), Modus
  Ponens(2, 3)

- 5. \(p_k \imp p_k\), Modus Ponens(1, 4)

- 6.
  \((p_k \imp p_k) \imp ( (p_k \imp p_k) \imp ( (p_k \imp p_k) \land (p_k \imp p_k)))\),
  Axiom \(J5\)

- 7. \((p_k \imp p_k) \imp ( (p_k \imp p_k) \land (p_k \imp p_k))\),
  Modus Ponens(5, 6)

- 8. \((p_k \imp p_k) \land (p_k \imp p_k)\), Modus Ponens(5, 7)

- 9. \((p_k \dimp p_k)\), Definition of \(\dimp\) (8)

Using the Axiom \(J6\) (or \(J7\)) we can introduce any number of
formulas to a theorem in \(J\). Hence, \(\vdash E_{n+1}\), thus
\(\phi(E_{n+1}) \in S_0\) according to our assumption of the existence
of a matrix \(M\). This however, entails that \(\phi(D_{n+1}) \in S_0\)
but that is a contradiction. ◻
